theories/test.v
@@ -2,3 +2,14 @@ From MetaCoq.Guarded Require Import plugin.
 From MetaCoq Require Import Utils.bytestring.
 
 Open Scope bs.
+
+Inductive rtree (X : Type) := rnode (l : list (rtree X)).
+
+Fixpoint rtree_size {X} (t : rtree X) := 
+  match t with
+  | rnode l => rnode X ((fix map (l : list (rtree X)) : list (rtree X) := match l with
+                                                                          | nil => nil
+                                                                          | cons a t => cons (rtree_size a) (map t)
+                                                                          end) l)
+  end.
+MetaCoq Run (check_fix_ci true (@rtree_size)). 
